Update parser interface
We now only have to handle cases where the parse trees use only valid
nonterminals.

This is important for the disjointness splitter, which uses the parser
itself (with the brute-force splitter) at refinement-time to check if a
rule accepts the empty string.

src/Common/List/Operations.v
@@ -1,5 +1,6 @@
 (** Useful list operations *)
 Require Import Coq.Lists.List.
+Require Import ADTSynthesis.Common.Equality.
 
 Set Implicit Arguments.
 
@@ -16,3 +17,61 @@ Fixpoint take {A} (n : nat) (ls : list A) : list A
        | _, nil => nil
        | S n', x::xs => x::take n' xs
      end.
+
+Definition disjoint {A} (eq_A : A -> A -> bool) (ls1 ls2 : list A) : bool
+  := fold_right
+       andb
+       true
+       (map
+          (fun x => negb (list_bin eq_A x ls2))
+          ls1).
+
+Lemma disjoint_bl {A eq_A} (lb : forall x y : A, x = y -> eq_A x y = true) ls1 ls2
+      (H : disjoint eq_A ls1 ls2 = true)
+: forall x, List.In x ls1 -> List.In x ls2 -> False.
+Proof.
+  unfold disjoint in *.
+  induction ls1; simpl in *; trivial.
+  apply Bool.andb_true_iff in H.
+  destruct H as [H0 H1].
+  specialize (IHls1 H1).
+  intros x [H'|H']; eauto; subst.
+  apply Bool.negb_true_iff, Bool.not_true_iff_false in H0.
+  specialize (fun k => H0 (list_in_lb lb k)); assumption.
+Defined.
+
+Lemma disjoint_lb {A eq_A} (bl : forall x y : A, eq_A x y = true -> x = y) ls1 ls2
+      (H : forall x, List.In x ls1 -> List.In x ls2 -> False)
+: disjoint eq_A ls1 ls2 = true.
+Proof.
+  unfold disjoint in *.
+  induction ls1; simpl in *; trivial.
+  rewrite IHls1 by intuition eauto.
+  rewrite Bool.andb_comm; simpl.
+  apply Bool.negb_true_iff, Bool.not_true_iff_false.
+  intro H'.
+  apply list_in_bl in H'; trivial; [].
+  intuition eauto.
+Defined.
+
+Lemma disjoint_comm {A eq_A}
+      ls1 ls2
+: disjoint (A := A) eq_A ls1 ls2 = disjoint (fun x y => eq_A y x) ls2 ls1.
+Proof.
+  unfold disjoint.
+  revert ls2.
+  induction ls1; simpl; trivial.
+  { induction ls2; eauto. }
+  { intro ls2.
+    rewrite IHls1; clear IHls1.
+    revert a ls1.
+    induction ls2; simpl; trivial.
+    { intros.
+      rewrite <- IHls2; simpl.
+      rewrite !Bool.negb_orb.
+      rewrite !Bool.andb_assoc.
+      repeat (f_equal; []).
+      rewrite <- !Bool.andb_assoc.
+      repeat (f_equal; []).
+      apply Bool.andb_comm. } }
+Qed.
