src/Parsers/BooleanRecognizerFull.v
@@ -1,0 +1,40 @@
+(** * Brute-force boolean recognizer *)
+Require Import Coq.Classes.RelationClasses.
+Require Import ADTSynthesis.Parsers.StringLike.String.
+Require Import ADTSynthesis.Parsers.BooleanRecognizer.
+Require Import ADTSynthesis.Parsers.ContextFreeGrammar.
+Require Import ADTSynthesis.Parsers.Splitters.RDPList ADTSynthesis.Parsers.Splitters.BruteForce.
+
+Set Implicit Arguments.
+
+Section example_parse_string_grammar.
+  Context (G : grammar Ascii.ascii).
+
+  Definition brute_force_parse_nonterminal
+  : @String Ascii.ascii _
+    -> String.string
+    -> bool
+    := let data := @brute_force_data Ascii.ascii _ G in parse_nonterminal (G := G).
+
+  Definition brute_force_parse_production
+             (str : @String Ascii.ascii _)
+  : production Ascii.ascii
+    -> bool
+    := let data := @brute_force_data Ascii.ascii _ G in parse_production (fun str' _ nt => brute_force_parse_nonterminal str' nt) (reflexivity str).
+
+  Definition brute_force_parse_productions
+             (str : @String Ascii.ascii _)
+  : productions Ascii.ascii
+    -> bool
+    := let data := @brute_force_data Ascii.ascii _ G in parse_productions (fun str' _ nt => brute_force_parse_nonterminal str' nt) (reflexivity str).
+
+  Definition brute_force_parse_item
+             (str : @String Ascii.ascii _)
+  : item Ascii.ascii
+    -> bool
+    := let data := @brute_force_data Ascii.ascii _ G in parse_item (fun nt => brute_force_parse_nonterminal str nt) str.
+
+  Definition brute_force_parse
+  : String.string -> bool
+    := fun str => brute_force_parse_nonterminal str G.
+End example_parse_string_grammar.
