src/Parsers/ParserImplementation.v
@@ -8,6 +8,7 @@ Require Import ADTSynthesis.Parsers.BaseTypes ADTSynthesis.Parsers.BooleanBaseTy
 Require Import ADTSynthesis.Parsers.StringLike.Core.
 Require Import ADTSynthesis.Parsers.MinimalParseOfParse.
 Require Import ADTSynthesis.Common.
+Require Import ADTSynthesis.Common.Equality.
 
 Set Implicit Arguments.
 
@@ -29,7 +30,7 @@ Section implementation.
     unfold rdp_list_is_valid_nonterminal in Hvalid; simpl in Hvalid.
     hnf in Hvalid.
     apply Equality.list_in_bl in Hvalid; [ | apply @Equality.string_bl ].
-    generalize (fun it its n pf pit pits prefix H' => @splits_for_complete Char G splitter str it its n pf pit pits (ex_intro _ nt (ex_intro _ prefix (conj Hvalid H')))).
+    generalize (fun it its n pf pit pits prefix H' pitH pitsH => @splits_for_complete Char G splitter str it its n pf (ex_intro _ nt (ex_intro _ prefix (conj Hvalid H'))) pit pits pitH pitsH).
     clear Hvalid.
     induction (G nt) as [ | x xs IHxs ].
     { intros; constructor. }
@@ -41,7 +42,7 @@ Section implementation.
         [ clear IHxs
         | apply IHxs;
           intros; eapply H'; try eassumption; [ right; eassumption ] ].
-      specialize (fun prefix it its H n pf pit pits => H' it its n pf pit pits prefix (or_introl H)).
+      specialize (fun prefix it its H n pf pit pits pitH pitsH => H' it its n pf pit pits prefix (or_introl H) pitH pitsH).
       clear -H'.
       induction x as [ | it its IHx ].
       { simpl; constructor. }
@@ -57,20 +58,69 @@ Section implementation.
         intros [ n [ pit pits ] ]; simpl in * |- .
         destruct (Compare_dec.le_ge_dec n (length str)).
         { exists n; repeat split; eauto.
+          specialize (fun pf =>
+                        H' _ pf
+                           (projT1 (parse_of_item__of__minimal_parse_of_item pit))
+                           (projT1 (parse_of_production__of__minimal_parse_of_production pits))).
           apply H'; eauto.
-          { exact (parse_of_item__of__minimal_parse_of_item pit). }
-          { exact (parse_of_production__of__minimal_parse_of_production pits). } }
+          { erewrite <- parse_of_item_respectful_refl.
+            eapply expand_forall_parse_of_item;
+              [ ..
+              | rewrite parse_of_item_respectful_refl;
+                exact (projT2 (parse_of_item__of__minimal_parse_of_item pit)) ];
+              try reflexivity; simpl.
+            simpl; intros ????? H0.
+            unfold rdp_list_is_valid_nonterminal in *.
+            apply list_in_bl in H0; [ | apply @string_bl ]; assumption. }
+          { erewrite <- parse_of_production_respectful_refl.
+            eapply expand_forall_parse_of_production;
+              [ ..
+              | rewrite parse_of_production_respectful_refl;
+                exact (projT2 (parse_of_production__of__minimal_parse_of_production pits)) ];
+              try reflexivity; simpl.
+            simpl; intros ????? H0.
+            unfold rdp_list_is_valid_nonterminal in *.
+            apply list_in_bl in H0; [ | apply @string_bl ]; assumption. } }
         { exists (length str).
           specialize (H' (length str) (reflexivity _)).
           pose proof (fun H => expand_minimal_parse_of_item (str' := take (length str) str) (reflexivity _) (reflexivity _) (or_introl (reflexivity _)) H pit) as pit'; clear pit.
           pose proof (fun H => expand_minimal_parse_of_production (str' := drop (length str) str) (reflexivity _) (reflexivity _) (or_introl (reflexivity _)) H pits) as pits'; clear pits.
           refine ((fun ret => let pit'' := pit' (fst (snd ret)) in
                               let pits'' := pits' (snd (snd ret)) in
-                              ((H' (fst (fst ret) pit'') (snd (fst ret) pits''), pit''), pits'')) _); repeat split.
-          { apply (@parse_of_item__of__minimal_parse_of_item Char splitter G _). }
-          { apply (@parse_of_production__of__minimal_parse_of_production Char splitter G _). }
+                              ((H' (projT1 (fst (fst ret) pit'')) (projT1 (snd (fst ret) pits'')) (projT2 (fst (fst ret) pit'')) (projT2 (snd (fst ret) pits'')), pit''), pits'')) _); repeat split.
+          { intro p.
+            exists (projT1 (@parse_of_item__of__minimal_parse_of_item Char splitter G _ _ _ _ _ p)).
+            erewrite <- parse_of_item_respectful_refl.
+            eapply expand_forall_parse_of_item;
+              [ ..
+              | rewrite parse_of_item_respectful_refl;
+                exact (projT2 (parse_of_item__of__minimal_parse_of_item p)) ];
+              try reflexivity; simpl.
+            simpl; intros ????? H0.
+            unfold rdp_list_is_valid_nonterminal in *.
+            apply list_in_bl in H0; [ | apply @string_bl ]; assumption. }
+          { intro p.
+            exists (projT1 (@parse_of_production__of__minimal_parse_of_production Char splitter G _ _ _ _ _ p)).
+            erewrite <- parse_of_production_respectful_refl.
+            eapply expand_forall_parse_of_production;
+              [ ..
+              | rewrite parse_of_production_respectful_refl;
+                exact (projT2 (parse_of_production__of__minimal_parse_of_production p)) ];
+              try reflexivity; simpl.
+            simpl; intros ????? H0.
+            unfold rdp_list_is_valid_nonterminal in *.
+            apply list_in_bl in H0; [ | apply @string_bl ]; assumption. }
           { rewrite !take_long; (assumption || reflexivity). }
           { apply bool_eq_empty; rewrite drop_length; omega. } } } }
+    Grab Existential Variables.
+    reflexivity.
+    reflexivity.
+    reflexivity.
+    reflexivity.
+    reflexivity.
+    reflexivity.
+    reflexivity.
+    reflexivity.
   Qed.
 
   Program Definition parser : Parser G splitter
