src/Parsers/SplitterFromParserADT.v
@@ -7,6 +7,7 @@ Require Import ADTSynthesis.Parsers.ParserInterface.
 Require Import ADTSynthesis.Parsers.ParserADTSpecification.
 Require Import ADTSynthesis.Parsers.StringLike.String.
 Require Import ADTSynthesis.Parsers.ContextFreeGrammarTransfer.
+Require Import ADTSynthesis.Parsers.ContextFreeGrammarTransferProperties.
 Require Import ADTSynthesis.ADTRefinement.Core.
 Require Import ADTSynthesis.Common ADTSynthesis.Common.Equality.
 
@@ -232,11 +233,14 @@ Section parser.
     end.
     lazymatch goal with
       | [ H : split_list_is_complete _ _ _ _ _, H' : ?n <= _,
-          p0 : parse_of_item _ _ _, p1 : parse_of_production _ _ _
+          p0 : parse_of_item _ _ _, p1 : parse_of_production _ _ _,
+          H'' : production_is_reachable _ _,
+          p0H : ContextFreeGrammarProperties.Forall_parse_of_item _ _,
+          p1H : ContextFreeGrammarProperties.Forall_parse_of_production _ _
           |- List.In ?n ?v ]
         => hnf in H;
           specialize (fun H0 H0' H1' =>
-                        H n H'
+                        H n H' H''
                           (@transfer_parse_of_item
                              Ascii.ascii adt_based_StringLike string_stringlike G
                              (fun s1 s2 => AbsR (projT2 splitter_impl) s2 (` s1))
@@ -244,8 +248,16 @@ Section parser.
                           (@transfer_parse_of_production
                              Ascii.ascii adt_based_StringLike string_stringlike G
                              (fun s1 s2 => AbsR (projT2 splitter_impl) s2 (` s1))
-                             H0 _ _ _ H1' p1));
-          apply H; clear H p0 p1; try assumption; simpl
+                             H0 _ _ _ H1' p1)
+                          (@transfer_forall_parse_of_item
+                             Ascii.ascii adt_based_StringLike string_stringlike G
+                             (fun s1 s2 => AbsR (projT2 splitter_impl) s2 (` s1))
+                             H0 _ _ _ _ H0' p0 p0H)
+                          (@transfer_forall_parse_of_production
+                             Ascii.ascii adt_based_StringLike string_stringlike G
+                             (fun s1 s2 => AbsR (projT2 splitter_impl) s2 (` s1))
+                             H0 _ _ _ _ H1' p1 p1H));
+          apply H; clear H p0H p1H p0 p1; try assumption; simpl
     end; [ split | | ];
     handle_rep;
     eauto with parser_adt_method_db.
